src/library/tactic/rewrite_tactic.h
@@ -5,7 +5,21 @@ Released under Apache 2.0 license as described in the file LICENSE.
 Author: Leonardo de Moura
 */
 #pragma once
+#include "library/tactic/apply_tactic.h"
 namespace lean {
+/*
+structure rewrite_cfg extends apply_cfg :=
+(md            := reducible)
+(symm          := ff)
+(occs          := occurrences.all)
+*/
+struct rewrite_cfg : public apply_cfg {
+    bool              m_symm{false};
+    occurrences       m_occs;
+    rewrite_cfg() { m_mode = transparency_mode::Reducible; }
+    rewrite_cfg(vm_obj const & cfg);
+};
+
 void initialize_rewrite_tactic();
 void finalize_rewrite_tactic();
 }
