tests/lean/run/kabstract_cache.lean
@@ -3,5 +3,5 @@ open tactic
 example {α : Type} (f : α → α → α) (a b : α) (H₁ : a = b) (H₂ : f b a = a) :
 let c := a in f c c = c :=
 by do dsimp,
-      get_local `H₁ >>= rewrite_core reducible tt tt (occurrences.pos [1]) ff,
+      e ← get_local `H₁, rewrite_target e {occs := occurrences.pos [1]},
       get_local `H₂ >>= exact
