tests/lean/run/rw1.lean
@@ -1,0 +1,84 @@
+namespace Ex1
+
+variables
+    (f : nat → nat → nat)
+    (p : nat → nat → Prop)
+    (h₁ : ∀ a b c, p b c → f a b = a)
+    (x y z : nat)
+    (h₂ : p y z)
+include f h₁ x y z h₂
+open tactic
+
+example : f x y = 0 + x :=
+begin
+  rw [h₁],
+  /- Resulting goals
+     ... ⊢ x = 0 + x
+     ... ⊢ p y ?m_1
+     ... ⊢ ℕ  -- This is ?m_1
+  -/
+  (do n ← num_goals, guard $ n = 3),
+  simp,
+  exact h₂
+end
+
+example : f x y = 0 + x :=
+begin
+  rw [h₁] {new_goals := new_goals.non_dep_only},
+  /- Resulting goals
+     ... ⊢ x = 0 + x
+     ... ⊢ p y ?m_1
+
+     ?m_1 is not included as a new goal because it occurs above.
+  -/
+  (do n ← num_goals, guard $ n = 2),
+  simp,
+  exact h₂
+end
+
+example : f x y = 0 + x :=
+begin
+  rw [h₁] {new_goals := new_goals.all},
+  /- Resulting goals
+     ... ⊢ x = 0 + x
+     ... ⊢ ℕ  -- This is ?m_1
+     ... ⊢ p y ?m_1
+
+     The order is preserved in this mode.
+  -/
+  (do n ← num_goals, guard $ n = 3),
+  simp,
+  exact z,
+  exact h₂
+end
+
+end Ex1
+
+namespace Ex2
+open tactic
+
+constant f : nat → nat
+constant p : nat → Prop
+/- The following lemma has an "auto_param", i.e., if `h` is not provided we
+   try to synthesize it using the `assumption` tactic -/
+lemma f_lemma (a : nat) (h : p a . assumption) : f a = a :=
+sorry
+
+/- `rw` has support for "auto_param"'s. -/
+example (x : nat) (h : p x) : f x = 0 + x :=
+begin
+  rw [f_lemma],
+  (do n ← num_goals, guard $ n = 1),
+  simp
+end
+
+/- We can disable auto_param support. -/
+example (x : nat) (h : p x) : f x = 0 + x :=
+begin
+  rw [f_lemma] {auto_param := ff},
+  (do n ← num_goals, guard $ n = 2),
+  simp,
+  exact h
+end
+
+end Ex2
