tests/lean/unfold1.lean
@@ -1,7 +1,8 @@
 open tactic
 
 meta definition rewriteH (Hname : name) : tactic unit :=
-do get_local Hname >>= rewrite_core reducible tt tt occurrences.all ff,
+do do h ← get_local Hname,
+   rewrite_target h,
    try reflexivity
 
 example (l : list nat) : list.append l [] = l :=
